{
 "cells": [
  {
   "cell_type": "markdown",
   "id": "0dc9f913",
   "metadata": {},
   "source": [
    "$\\newcommand\\indep{\\perp}$\n",
    "$\\newcommand\\and{\\cap}$\n",
    "$\\newcommand\\or{\\cup}$\n",
    "$\\newcommand\\implies{\\Rightarrow}$\n",
    "$\\newcommand\\var{\\mathbb{V}ar}$\n",
    "$\\newcommand\\E{\\mathbb{E}}$"
   ]
  },
  {
   "cell_type": "markdown",
   "id": "f2427346",
   "metadata": {},
   "source": [
    "# Chapter 2: Foundations"
   ]
  },
  {
   "cell_type": "markdown",
   "id": "67162c61",
   "metadata": {},
   "source": [
    "### Exercise 2.1\n",
    "\n",
    "a. Prove that $P(\\emptyset) = 0$\n",
    "\n",
    "From definition 2.1 we know that\n",
    "\n",
    "$$\n",
    "\\text{If } \\alpha, \\beta \\in \\mathcal{S} \\text{ and } \\alpha \\and \\beta = \\emptyset, \\text{ then } P(\\alpha \\or \\beta) = P(\\alpha) + P(\\beta)\n",
    "$$\n",
    "\n",
    "Taking $\\alpha = \\Omega$ and $\\beta = \\emptyset$ and combining with the facts that $P(\\Omega) = 1$, $\\Omega \\and \\emptyset = \\emptyset$ (nothing intersects with $\\emptyset$), and $\\Omega \\or \\emptyset = \\Omega$ ($\\Omega$ is the set of all possible outcomes) we have\n",
    "\n",
    "$$\n",
    "P(\\Omega \\or \\emptyset) = P(\\Omega) + P(\\emptyset), \\\\\n",
    "\\implies P(\\Omega) = P(\\Omega) + P(\\emptyset), \\\\\n",
    "\\implies P(\\emptyset) = 0.\n",
    "$$\n",
    "\n",
    "\n",
    "\n",
    "b. Prove that if $\\alpha \\subseteq \\beta$, then $P(\\alpha) \\leq P(\\beta)$.\n",
    "\n",
    "According to the frequentist interpretation of probabilities, \n",
    "\n",
    "$$\n",
    "P(\\alpha) = \\frac{|\\alpha|}{|\\mathcal{S}|}\n",
    "$$\n",
    "\n",
    "Thus, if $\\alpha \\subseteq \\beta$, then,\n",
    "$$\n",
    "|\\alpha| \\leq |\\beta|, \\\\\n",
    "\\implies \\frac{|\\alpha|}{|\\mathcal{S}|} \\leq \\frac{|\\beta|}{|\\mathcal{S}|}, \\\\\n",
    "\\implies P(alpha) \\leq P(beta).\n",
    "$$\n",
    "\n",
    "\n",
    "c. Prove that $P(\\alpha \\or \\beta) = P(\\alpha) + P(\\beta) - P(\\alpha \\and \\beta)$.\n",
    "\n",
    "We know that $P(\\alpha \\or \\beta) = P(\\alpha) + P(\\beta)$ when $\\alpha$ and $\\beta$ are disjoint sets with $\\alpha \\and \\beta = \\emptyset$.\n",
    "\n",
    "Expressing $\\alpha \\or \\beta$ as the union of disjoint sets:\n",
    "$$\n",
    "\\alpha \\or \\beta = \\alpha \\or (\\beta \\and \\overline{\\alpha}), \\\\\n",
    "\\implies P(\\alpha \\or \\beta) = P(\\alpha) + P(\\beta \\and \\overline{\\alpha}).\n",
    "$$\n",
    "Also expressing $\\beta$ as the union of disjoint sets:\n",
    "$$\n",
    "\\beta = (\\alpha \\and \\beta) \\or (\\beta \\and \\overline{\\alpha}), \\\\\n",
    "\\implies P(\\beta) = P(\\alpha \\and \\beta) + P(\\beta \\and \\overline{\\alpha}), \\text{ or} \\\\\n",
    "P(\\beta \\and \\overline{\\alpha}) = P(\\beta) - P(\\alpha \\and \\beta).\n",
    "$$\n",
    "Substituting the value of $P(\\beta \\and \\overline{\\alpha})$ into the first equation, we have,\n",
    "$$\n",
    "P(\\alpha \\or \\beta) = P(\\alpha) + P(\\beta \\and \\overline{\\alpha}), \\\\\n",
    "\\implies P(\\alpha \\or \\beta) = P(\\alpha) + P(\\beta) - P(\\alpha \\and \\beta).\n",
    "$$"
   ]
  },
  {
   "cell_type": "markdown",
   "id": "4b7ecc05",
   "metadata": {},
   "source": [
    "### Exercise 2.2\n",
    "\n",
    "a. Show that for binary random variables $X$, $Y$ , the event-level independence $(x^0 \\indep y^0)$ implies random variable independence $(X \\indep Y )$.\n",
    "\n",
    "As per the definition of independence, $\\alpha \\indep \\beta$ iff $P(\\alpha \\and \\beta) = P(\\alpha)(\\beta)$. So, \n",
    "$$\n",
    "(x^0 \\indep y^0) \\implies P(x^0 \\and y^0) = P(x^0)(y^0).\n",
    "$$\n",
    "\n",
    "Consider,\n",
    "\n",
    "b. Show a counterexample for nonbinary variables.\n",
    "\n",
    "c. Is it the case that, for a binary-valued variable $Z$, we have that $(X \\indep Y | z^0)$ implies $(X \\indep Y | Z)$ ?"
   ]
  },
  {
   "cell_type": "markdown",
   "id": "b08af29c",
   "metadata": {},
   "source": [
    "### Exercise 2.5\n",
    "\n",
    "Let $X$, $Y$ , $Z$ be three disjoint subsets of variables such that $\\chi = X \\or Y \\or Z$. Prove that $P |= (X \\indep Y | Z)$ if and only if we can write $P$ in the form:\n",
    "\n",
    "$$\n",
    "P(\\chi) = \\phi_{1}(X,Z)\\phi_{2}(Y,Z).\n",
    "$$\n",
    "\n",
    "We need to prove that \n",
    "$$\n",
    "X \\indep Y | Z  \\iff P(\\chi) = \\phi_{1}(X,Z)\\phi_{2}(Y,Z).\n",
    "$$\n",
    "\n",
    "Sufficiency (LHS implies RHS):\n",
    "\n",
    "We know, $X \\indep Y | Z \\implies P(X \\and Y | Z) = P(X | Z) P(Y | Z)$\n",
    "\n",
    "So, we start with $P(X \\and Y | Z)$:\n",
    "$$\n",
    "P(X,Y|Z) = \\frac{P(X,Y,Z)}{P(Z)} = \\frac{P(\\chi)}{P(Z)} \\\\\n",
    "= \\frac{P(\\chi)}{\\iint (x,y,Z) dx dy}  \\cdots \\text{Due to marginalization property} \\\\\n",
    "= \\frac{P(\\chi)}{\\int \\phi_{1}(x,Z) dx \\int \\phi_{2}(x,Y) dy} \\cdots \\text{X and Y are disjoint and can be factorized} \\\\\n",
    "= \\frac{\\phi_{1}(X,Z)}{\\int \\phi_{1}(x,Z) dx} \\cdot \\frac{\\phi_{2}(Y,Z)}{\\int \\phi_{2}(y,Z) dy} \\cdots \\text{Again, as the variables are disjoint, they can be factorized.}\n",
    "$$\n",
    "\n",
    "So $P(X,Y|Z)$ can be factorized, so $(X \\indep Y | Z)$.\n",
    "\n",
    "Necessity (RHS implies LHS):\n",
    "\n",
    "$$\n",
    "P(\\chi) = P(X,Y,Z) = P(X | Y,Z) P(Y,Z) \\\\\n",
    "= P(X|Z) P(Y,Z) \\cdots \\text{We have assumed LHS to be true, i.e. $(X \\indep Y | Z)$.}\n",
    "$$\n",
    "\n",
    "The first and second terms could be represented as $\\phi_{1}$ and $\\phi_{2}$ respectively."
   ]
  },
  {
   "cell_type": "markdown",
   "id": "1ca0ac3f",
   "metadata": {},
   "source": [
    "### Exercise 2.7\n",
    "\n",
    "In this exercise, you will prove the properties of conditional independence discussed in section 2.1.4.3.\n",
    "\n",
    "a. Prove that the weak union and contraction properties hold for any probability distribution $P$.\n",
    "\n",
    "b. Prove that the intersection property holds for any positive probability distribution $P$.\n",
    "\n",
    "c. Provide a counterexample to the intersection property in cases where the distribution $P$ is not positive.\n",
    "\n",
    "\n",
    "a. **Proving weak union**\n",
    "\n",
    "To prove:\n",
    "\n",
    "$$\n",
    "(X \\indep Y , W | Z) \\implies (X \\indep Y | Z, W ).\n",
    "$$\n",
    "\n",
    "We prove by considering the different possible cases. \n",
    "\n",
    "If $P(Z,W) = 0$ then by definition of marginal independence, $(X \\indep Y | Z, W)$. If $P(Z) = 0$ then $P(Z,W) = 0$ and thus $(X \\indep Y | Z, W)$ is true again. \n",
    "\n",
    "If $P(Z) \\neq 0$ and $P(Z,W) \\neq 0$:\n",
    "Assume the LHS is true, i.e. \n",
    "\n",
    "$$\n",
    "P(X,Y,W | Z) = P(X|Z)P(Y,W|Z), \\cdots \\text{(1)}\n",
    "$$\n",
    "\n",
    "So, we need to prove given the above is true, the following is also true:\n",
    "\n",
    "$$\n",
    "P(X,Y|Z,W) = P(X|Z,W)P(Y|Z,W).\n",
    "$$\n",
    "\n",
    "Starting from the LHS of the above expression:\n",
    "\n",
    "$$\n",
    "P(X,Y|Z,W) = \\frac{P(X,Y,W|Z)}{P(W|Z)} \\cdots \\text{by Baye's rule and chain rule}. \\\\\n",
    "= \\frac{P(X|Z)P(Y,W|Z)}{P(W|Z)} \\cdots \\text{from our assumption in (1).} \\\\\n",
    "= P(X|Z)P(Y|Z,W). \\cdots \\text{(2)}\n",
    "$$\n",
    "\n",
    "Now, we know from the decomposition property,\n",
    "\n",
    "$$\n",
    "(X \\indep Y , W | Z) \\implies (X \\indep Y | Z) \\implies (X \\indep W | Z).\n",
    "$$\n",
    "\n",
    "So,\n",
    "\n",
    "$$\n",
    "P(X|Z) = P(X|W,Z).\n",
    "$$\n",
    "\n",
    "So, we can rewrite the result (2) as\n",
    "\n",
    "$$\n",
    "P(X,Y|Z,W) = P(X|Z)P(Y|Z,W) = P(X|Z,W)P(Y|Z,W),\n",
    "$$\n",
    "\n",
    "which is what is needed to prove.\n",
    "\n",
    "\n",
    "\n",
    "**Proving contraction**\n",
    "\n",
    "To prove:\n",
    "\n",
    "$$\n",
    "(X \\indep W | Z, Y ) \\& (X \\indep Y | Z) \\implies (X \\indep Y , W | Z). \\cdots \\text{(1)}\n",
    "$$\n",
    "\n",
    "Again, trivially, if $P(Z) = 0$, $X \\indep Y, W | Z$ holds. \n",
    "\n",
    "Now, assuming the LHS of (1) is true. We can infer,\n",
    "\n",
    "$$\n",
    "(X \\indep W | Z,Y) \\implies P(X,W|Z,Y) = P(X|Z,Y)P(W|Z,Y) \\cdots \\text{(2)}.\n",
    "$$\n",
    "\n",
    "Now, we need to prove \n",
    "\n",
    "$$\n",
    "(X \\indep Y,W | Z), \\text{or}, \\\\\n",
    "P(X,Y,W|Z) = P(X|Z)P(Y,W|Z) \\cdots \\text{(3)}\n",
    "$$\n",
    "\n",
    "Starting from the LHS of (3),\n",
    "\n",
    "$$\n",
    "P(X,Y,W|Z) = P(X,W|Z,Y)P(Y|Z) \\\\\n",
    "= P(X|Z,Y)P(W|Z,Y)P(Y|Z) \\cdots \\text{from (2)} \\\\\n",
    "= P(X|Z)P(W|Z,Y)P(Y|Z) \\cdots \\text{from the assumption that $X \\indep Y | Z$.} \\\\\n",
    "= P(X|Z)P(Y,W|Z) \\cdots \\text{from the chain rule},\n",
    "$$\n",
    "\n",
    "which completes our proof.\n",
    "\n",
    "\n",
    "\n",
    "b. **Proving intersection**\n",
    "\n",
    "To prove:\n",
    "\n",
    "$$\n",
    "(X \\indep Y | Z, W ) \\& (X \\indep W | Z, Y ) \\implies (X \\indep Y , W | Z) \\\\\n",
    "\\text{for $P(\\alpha) \\gt 0$}.\n",
    "$$\n",
    "\n",
    "Using the proof for contraction again, we need to prove \n",
    "\n",
    "$$\n",
    "(X \\indep Y,W | Z), \\text{or}, \\\\\n",
    "P(X,Y,W|Z) = P(X|Z)P(Y,W|Z) \\cdots \\text{(1)}\n",
    "$$\n",
    "\n",
    "Starting from the LHS of (1),\n",
    "\n",
    "$$\n",
    "P(X,Y,W|Z) = P(X,W|Z,Y)P(Y|Z) \\\\\n",
    "= P(X|Z,Y)P(W|Z,Y)P(Y|Z) \\cdots \\text{given} \\\\\n",
    "= P(X|Z,Y)P(W|Z,Y)P(Y|Z) \\cdots \\\\\n",
    "= P(X|Z,Y)P(Y,W|Z) \\cdots \\text{(2)}.\n",
    "$$\n",
    "\n",
    "Now, if we prove that $X \\indep Y | Z$ we can say, $P(X|Z,Y) = P(X|Z)$.Thus,\n",
    "\n",
    "$$\n",
    "P(X|Z) = \\sum_{w \\in W} P(X,w|Z) \\\\\n",
    "= \\sum_{w \\in W} P(X|w,Z)P(w|Z) \\\\\n",
    "= \\sum_{w \\in W} P(X|Y,w,Z)P(w|Z) \\cdots \\text{since (X \\indep Y | W,Z)} \\\\\n",
    "= \\sum_{w \\in W} P(X|Y,Z)P(w|Z) \\cdots \\text{since (X \\indep W | Y, Z)} \\\\\n",
    "= P(X|Y,Z) \\sum_{w \\in W} P(w|Z) \\\\\n",
    "= P(X|Y,Z) \\cdots \\text{Due the marginalization}.\n",
    "$$\n",
    "\n",
    "This shows that $X \\indep Y | Z$. Thus (2) can be written as:\n",
    "\n",
    "$$\n",
    "P(X,Y,W|Z) = P(X|Z)P(Y,W|Z)\n",
    "$$\n",
    "\n",
    "or,\n",
    "\n",
    "$$\n",
    "(X \\indep Y , W | Z).\n",
    "$$\n",
    "\n"
   ]
  },
  {
   "cell_type": "markdown",
   "id": "5cbe4aff",
   "metadata": {},
   "source": [
    "### Exercise 2.11\n",
    "\n",
    "Use the properties of expectation to show that we can rewrite the variance of a random variable X as\n",
    "\n",
    "$$\n",
    "\\var[X] = \\E[X^2] - (\\E[X])^2\n",
    "$$\n",
    "\n",
    "From the definition of variance,\n",
    "\n",
    "$$\n",
    "\\E[(X - \\E[X])^2] \\\\\n",
    "= \\E[X^2 - 2X\\E[X] + (\\E[X])^2] \\\\\n",
    "= \\E[X^2] - \\E[2X\\E[X]] + \\E[(\\E[X])^2] \\cdots \\text{By the linearity of expectation.} \\\\\n",
    "= \\E[X^2] + (\\E[X])^2 - 2\\E[X]\\E[X] \\cdots \\text{$\\E[\\E[X]] = \\E[X]$} \\\\\n",
    "= \\E[X^2] + (\\E[X])^2 - 2(\\E[X])^2 \\\\\n",
    "= \\E[X^2] - (\\E[X])^2. \n",
    "$$"
   ]
  },
  {
   "cell_type": "markdown",
   "id": "2822c30b",
   "metadata": {},
   "source": [
    "### Exercise 2.12\n",
    "\n",
    "**Markov inequality**\n",
    "\n",
    "Let $X$ be a random variable such that $P(X â‰¥ 0) = 1$, then for any $t \\ge 0$,\n",
    "\n",
    "$$\n",
    "P(X \\ge t) \\le \\frac{\\E_{P}[X]}{t}.\n",
    "$$\n",
    "\n",
    "We know,\n",
    "\n",
    "$$\n",
    "\\E[X] = \\int_{-\\infty}^{\\infty} x P(x) dx. = \\int_{0}^{\\infty} x P(x) dx \\cdots \\text{$X$ is non-negative} \\\\\n",
    "= \\int_{0}^{t} x P(x) dx + \\int_{t}^{\\infty} x P(x) dx \\ge \\int_{t}^{\\infty} x P(x) dx \\ge \\int_{t}^{\\infty} t P(x) dx \\cdots \\text{we are considering the range where $x \\ge t$} \\\\\n",
    "\\ge t \\int_{t}^{\\infty} P(x) dx = t P(X \\ge t). \\\\\n",
    "\\text{Thus,} \\E[X] \\ge t P(X \\ge t) \\text{or,} \\\\\n",
    "P(X \\ge t) \\le \\frac{\\E_{P}[X]}{t} \\cdots \\text{Proved.}\n",
    "$$"
   ]
  },
  {
   "cell_type": "code",
   "execution_count": null,
   "id": "3c7e8c0b",
   "metadata": {},
   "outputs": [],
   "source": []
  }
 ],
 "metadata": {
  "kernelspec": {
   "display_name": "Python 3 (ipykernel)",
   "language": "python",
   "name": "python3"
  },
  "language_info": {
   "codemirror_mode": {
    "name": "ipython",
    "version": 3
   },
   "file_extension": ".py",
   "mimetype": "text/x-python",
   "name": "python",
   "nbconvert_exporter": "python",
   "pygments_lexer": "ipython3",
   "version": "3.7.12"
  }
 },
 "nbformat": 4,
 "nbformat_minor": 5
}
